Disj.v
@@ -74,14 +74,6 @@ Proof.
       cbn in IHl3. right. firstorder.
 Qed.
 
-Lemma disjoint2 {A : Type} `{EqDec A} (l1 l2 : list A)
-  : Disjoint l1 l2 <-> forall x y, x ∈ l1 -> y ∈ l2 -> x <> y.
-Proof.
-  split;unfold Disjoint;intros.
-  - intro N. subst x. firstorder.
-  - split;intros;intro N;eapply H0;eauto.
-Qed.
-
 Local Arguments deq_loop {_ _ _ _ _}.
 Arguments loop_head {_ _ _ _ _}.
 Arguments loop_head_dec {_ _ _ _ _}.
